Proof of single-step noninterference with one call
This is a proof of a single step of noninterference without downgrades,
sometimes referred to as "the unwinding condition" in a formal
verification context, or "single command noninterference" in a
programming languages context. This means that if we run the state
transition function for just one step, then noninterference is enforced for
that one step. At the moment, the model just has a single call that is
actually properly modeled (the write call), so this is not really a complete
proof. The definition of noninterference is also still undergoing revision.
The proof itself is also not terribly automated and almost no effort was
put into making it elegent yet.

experimental/ni_coq/vfiles/GenericMap.v
@@ -4,16 +4,32 @@ From Coq Require Import Logic.FunctionalExtensionality.
 
 Class KeyT:= {
     t: Type;
-    eqb: t -> t -> bool
+    eq_dec: forall (t1 t2: t), {t1 = t2} + {t1 <> t2};
     (* TODO, undoubtedly proof obligations *)
 }.
+
+Theorem eq_key {KT: KeyT}: forall (T: Type) (k: t) (p q: T),
+    (if (eq_dec k k) then p else q) = p.
+Proof. 
+    intros. destruct (eq_dec k k).
+    reflexivity. 
+    exfalso. apply n. reflexivity.
+Qed.
+
+Theorem neq_key {KT: KeyT}: forall (T: Type) (k1 k2: t) (p q: T),
+    k1 <> k2 ->
+    (if (eq_dec k1 k2) then p else q) = q.
+Proof. 
+    intros. destruct (eq_dec k1 k2).
+    contradiction. reflexivity.
+Qed.
 
 Definition tg_map (KT: KeyT)(VT: Type) := t -> VT.
 Definition tg_empty {KT: KeyT}{VT: Type}(def: VT): tg_map KT VT :=
     (fun _ => def).
 Definition tg_update {KT: KeyT}{VT: Type}(m: tg_map KT VT)
     (k: t)(v: VT) :=
-    fun k' => if eqb k k' then v else m k'.
+    fun k' => if eq_dec k k' then v else m k'.
 
 Definition tg_fmap {KT: KeyT}{VT: Type}
     (f: VT -> VT)(m: tg_map KT VT): tg_map KT VT :=
@@ -23,6 +39,22 @@ Notation "'_' '!->' v" := (tg_empty v)
   (at level 100, right associativity).
 Notation "x '!->' v ';' m" := (tg_update m x v)
   (at level 100, v at next level, right associativity).
+
+Theorem upd_eq {KT: KeyT}{VT: Type}: forall (m: tg_map KT VT) k v,
+    (k !-> v; m) k = v.
+Proof.
+    intros. unfold tg_update. rewrite eq_key. reflexivity.
+Qed.
+
+
+Theorem upd_neq {KT: KeyT}{VT: Type}: forall (m: tg_map KT VT) k1 k2 v,
+    (k1 <> k2) ->
+    (k1 !-> v; m) k2 = (m k2).
+Proof.
+    intros. unfold tg_update. rewrite neq_key. reflexivity.
+    apply H.
+Qed.
+    
 
 Definition pg_map (KT: KeyT)(VT: Type) :=
     tg_map KT (option VT).
